done libs, next tube.fst

test/tube/IO.h
@@ -1,0 +1,78 @@
+#ifndef FSTAR_IO
+#define FSTAR_IO
+//#define _POSIX_C_SOURCE 199309L
+//#define _BSD_SOURCE
+//#define _DEFAULT_SOURCE
+//#define _GNU_SOURCE
+
+#include <time.h>
+#include <sys/types.h>
+#include <sys/stat.h>
+#include <fcntl.h>
+#include <unistd.h>
+#include <sys/mman.h>
+#include <sys/socket.h>
+#include <netinet/in.h>
+#include <netdb.h>
+#include <stdio.h>
+#include <string.h>
+#include <strings.h>
+#include <stdint.h>
+#include <stdlib.h>
+#include <errno.h>
+#include <arpa/inet.h> 
+#include "testlib.h"
+
+typedef enum {FileOk, FileError} PaddedFileIO_fresult;
+typedef enum {FileOpen, FileClosed} PaddedFileIO_fd_state;
+
+typedef struct {
+  uint64_t current;
+  uint8_t* buf;
+} PaddedFileIO_mmap;
+
+typedef struct {
+  int fd;
+  uint64_t current;
+  uint8_t* mmap;
+  uint8_t* last;
+} PaddedFileIO_file_descriptor;
+
+typedef struct {
+  uint8_t* name;
+  uint64_t mtime;
+  uint64_t size;
+} PaddedFileIO_file_stat;
+
+typedef struct {
+  PaddedFileIO_file_stat stat;
+  PaddedFileIO_file_descriptor fd;
+} PaddedFileIO_file_handle;
+
+
+#define PaddedFileIO_max_block_size (256 * 1024)
+
+PaddedFileIO_fresult PaddedFileIO_file_open_read_sequential(uint8_t* file, PaddedFileIO_file_handle* fh);
+PaddedFileIO_fresult PaddedFileIO_file_open_write_sequential(PaddedFileIO_file_stat st, PaddedFileIO_file_handle* fh);
+uint8_t* PaddedFileIO_file_next_read_buffer(PaddedFileIO_file_handle* fh,uint64_t len);
+uint8_t* PaddedFileIO_file_next_write_buffer(PaddedFileIO_file_handle* fh,uint64_t len);
+PaddedFileIO_fresult PaddedFileIO_file_close(PaddedFileIO_file_handle* fh);
+
+
+typedef enum {SocketOk, SocketError} SocketIO_sresult;
+
+typedef struct {
+  int fd;
+  uint64_t sent_bytes;
+  uint64_t received_bytes;
+} SocketIO_socket;
+
+
+SocketIO_sresult SocketIO_tcp_connect(char* host, int port, SocketIO_socket* sh);
+SocketIO_sresult SocketIO_tcp_listen(int port, SocketIO_socket* sh);
+SocketIO_sresult SocketIO_tcp_accept(SocketIO_socket* lh, SocketIO_socket* conn);
+SocketIO_sresult SocketIO_tcp_write_all(SocketIO_socket* conn, uint8_t* buf, uint64_t len);
+SocketIO_sresult SocketIO_tcp_read_all(SocketIO_socket* conn, uint8_t* buf, int len);
+SocketIO_sresult SocketIO_tcp_close(SocketIO_socket* conn);
+
+#endif
