test/tube/SocketIO.c
@@ -1,0 +1,114 @@
+#include "IO.h"
+
+
+SocketIO_sresult SocketIO_tcp_connect(char* host, int port, SocketIO_socket* sh) {
+  int sockfd = 0, n = 0;
+  struct sockaddr_in serv_addr; 
+  if((sockfd = socket(AF_INET, SOCK_STREAM, 0)) < 0)
+    {
+      perror("Error : Could not create socket");
+      return SocketError;
+    } 
+
+  struct hostent *server = gethostbyname(host);
+  if (server == NULL) {
+    perror("SocketError, DNS lookup on host failed");
+    return SocketError;
+  }
+  memset(&serv_addr, '0', sizeof(serv_addr)); 
+  serv_addr.sin_family = AF_INET;
+  serv_addr.sin_port = htons(port); 
+  bcopy((char *)server->h_addr, 
+	(char *)&serv_addr.sin_addr.s_addr, server->h_length);
+  /*
+  if(inet_pton(AF_INET, host, &serv_addr.sin_addr)<=0)
+    {
+      perror("inet_pton error occured");
+      return SocketError;
+    } 
+  */
+  if( connect(sockfd, (struct sockaddr *)&serv_addr, sizeof(serv_addr)) < 0)
+    {
+      perror("Error : Connect Failed");
+      return SocketError;
+    } 
+  sh->fd = sockfd;
+  sh->sent_bytes = 0;
+  sh->received_bytes = 0;
+  return SocketOk;
+}
+
+SocketIO_sresult SocketIO_tcp_listen(int port, SocketIO_socket* sh) {
+  int listenfd = 0;
+  struct sockaddr_in serv_addr; 
+
+  if((listenfd = socket(AF_INET, SOCK_STREAM, 0)) < 0)
+    {
+      perror("Error : Could not create socket");
+      return SocketError;
+    } 
+  memset(&serv_addr, '0', sizeof(serv_addr)); 
+  serv_addr.sin_family = AF_INET;
+  serv_addr.sin_addr.s_addr = htonl(INADDR_ANY);
+  serv_addr.sin_port = htons(port); 
+
+  if (bind(listenfd, (struct sockaddr*)&serv_addr, sizeof(serv_addr)) < 0) {
+    perror("bind");
+    return SocketError;
+  }
+    
+  if (listen(listenfd, 10) < 0) {
+    perror("listen");
+    return SocketError;
+  }
+  sh->fd = listenfd;
+  return SocketOk;
+}
+
+SocketIO_sresult SocketIO_tcp_accept(SocketIO_socket* lh, SocketIO_socket* conn) {
+  int sockfd = 0;
+  sockfd = accept(lh->fd, (struct sockaddr*)NULL, NULL); 
+  if( sockfd < 0)
+    {
+      perror("Error : accept Failed");
+      return SocketError;
+    } 
+  conn->fd = sockfd;
+  return SocketOk;
+}
+
+
+SocketIO_sresult SocketIO_tcp_write_all(SocketIO_socket* conn, uint8_t* buf, uint64_t len) {
+  if (write(conn->fd, buf, len) < len) {
+    perror("write did not write all");
+    return SocketError;
+  }
+  conn->sent_bytes += len;
+  return SocketOk;
+}    
+
+
+SocketIO_sresult SocketIO_tcp_read_all(SocketIO_socket* conn, uint8_t* buf, int len) {
+  int got = 0;
+  while (got < len) {
+    int n = read(conn->fd, buf+got, len-got);
+    if (n == 0) {
+      perror("early end of file");
+      return SocketError;
+    }
+    if (n < 0) {
+      perror("socket read error");
+      return SocketError;
+    }
+    got += n;
+  }
+  conn->received_bytes += got;
+  return SocketOk;
+}
+
+SocketIO_sresult SocketIO_tcp_close(SocketIO_socket* conn) {
+  shutdown(conn->fd,2);
+  printf("Sent %llu bytes, Received %llu bytes\n",conn->sent_bytes,conn->received_bytes);
+  return SocketOk;
+}
+
