test/tube/Hacl.Tube.fst
@@ -3,7 +3,7 @@ module Hacl.Tube
 
 open FStar.Seq
 open FStar.Buffer
-open SecureFileIO
+open PaddedFileIO
 open SocketIO
 open Hacl.Constants
 
@@ -14,18 +14,15 @@ type string = seq u8
 type streamID = {
      id: u64;
      ts: u64;
+}
+
+type principals = {
      pkA: seq u8;
      pkB: seq u8
 }
 
-     
-type event : Type0 = 
-    | Sent: sid:streamID -> header:file_stat -> content: seq u8 -> event
 
-assume val happened: FStar.HyperStack.mem -> event -> GTot bool
-assume val log: e:event -> Stack unit
-    (requires (fun _ -> True))
-    (ensures  (fun h0 s h1 -> happened h1 e))
+assume val sent: FStar.HyperStack.mem -> principals -> streamID -> file_stat -> (seq u8) -> GTot bool
 
 assume val file_send: file:string -> roundup:u64 ->
        host:string -> port:u32 -> 
@@ -34,17 +31,23 @@ assume val file_send: file:string -> roundup:u64 ->
 	   (requires (fun _ -> True))
 	   (ensures  (fun h0 s h1 -> match s with 
       	   	                   | FileOk,fs,sid ->
-				     sid.pkA = as_seq h0 pkA /\	sid.pkB = as_seq h0 pkB /\
+				     let prins = {pkA = as_seq h0 pkA; pkB = as_seq h0 pkB} in
 				     file_content h0 fs = file_content h1 fs /\	
-				     happened h1 (Sent sid fs (as_seq h0 (file_content h0 fs)))
+				     sent h1 prins sid fs (file_content h0 fs)
 				   | _ -> true))
 
 assume val file_recv: port:u32 -> pkA:buffer u8 -> skB:buffer u8 -> pkB:buffer u8 -> Stack (fresult * file_stat * streamID)
        	   (requires (fun _ -> True))
 	   (ensures  (fun h0 s h1 -> match s with 
       	   	                   | FileOk,fs,sid ->
-				     sid.pkA = as_seq h0 pkA /\	sid.pkB = as_seq h0 pkB /\
-				     happened h0 (Sent sid fs (as_seq h1 (file_content h1 fs)))
+				     let prins = {pkA = as_seq h0 pkA; pkB = as_seq h0 pkB} in
+				     sent h0 prins sid fs (file_content h1 fs)
 				   | _ -> true))
 
 
+
+val main: unit -> ST FStar.Int32.t
+  (requires (fun h -> True))
+  (ensures  (fun h0 r h1 -> True))
+let main () =
+  C.exit_success
