test/tube/PaddedFileIO.fsti
@@ -1,0 +1,116 @@
+module PaddedFileIO
+
+open FStar.Seq
+open FStar.Buffer
+open Hacl.Cast
+open Hacl.Constants
+open Hacl.UInt64
+
+(* Need to get rid of these  following ones *)
+type string = seq u8
+val zero: u64
+val sub: buffer u8 -> u64 -> u64 -> Tot (buffer u8)
+val v: u64 -> Tot nat
+(* The above need to come from some library module *)
+
+(* File System Buffer Size, currently 256KB *)
+val max_block_size: u64
+
+
+type file_stat: Type0 = {
+     name: uint8_p;
+     mtime: h64;
+     size: h64;	
+}
+
+val file_descriptor: Type0
+
+type fd_state = 
+     | FileOpen: fd_state
+     | FileClosed: fd_state
+
+type file_handle: Type0 =  {
+     stat:   file_stat;
+     fd:     file_descriptor
+}
+
+type fresult : Type0 = 
+     | FileOk    : fresult
+     | FileError : fresult
+
+
+val file_state: FStar.HyperStack.mem -> file_handle -> GTot fd_state
+val file_offset: FStar.HyperStack.mem -> file_handle -> GTot u64
+val file_buffer: FStar.HyperStack.mem -> file_stat -> GTot (buffer u8)
+val file_content: FStar.HyperStack.mem -> file_stat -> GTot (seq u8)
+
+let file_sub (m:FStar.HyperStack.mem) (f:file_handle) (i:u64) (j:u64) =	
+    sub (file_buffer m f.stat) i j
+    
+
+(* TODO: check the live/modifies clauses below *)
+val file_open_read_sequential: n:uint8_p -> fb:buffer file_handle -> Stack fresult
+    (requires (fun h -> length fb = 1 /\ live h fb))
+    (ensures  (fun h0 s h1 -> match s with 
+	      	       	    | FileOk -> 
+			      live h1 fb /\
+			      modifies_1 fb h0 h1 /\
+			      (let fh = get h1 fb 0 in
+    	      	     	       file_state h1 fh = FileOpen /\	
+			       file_offset h1 fh = zero /\	
+			       file_content h0 fh.stat = file_content h1 fh.stat)
+			    | _ -> true))
+
+
+val file_open_write_sequential: file_stat -> fb:buffer file_handle -> Stack fresult
+    (requires (fun h -> length fb = 1 /\ live h fb))
+    (ensures  (fun h0 s h1 -> match s with 
+    	      	      	    | FileOk -> 
+			      live h1 fb /\
+			      (let fh = get h1 fb 0 in
+    	      	      	       file_state h1 fh = FileOpen /\ 
+			       file_offset h1 fh = zero /\
+			       file_content h0 fh.stat = file_content h1 fh.stat)
+			    | _ -> true))
+
+val file_next_read_buffer: fb:buffer file_handle -> len:u64 -> Stack uint8_p
+    (requires (fun h0 -> v len <= v max_block_size /\
+    	      	         length fb = 1 /\ live h0 fb /\
+    	      	         (let f = get h0 fb 0 in
+			  file_state h0 f = FileOpen)))
+    (ensures  (fun h0 s h1 -> let f = get h1 fb 0 in
+    	      	              let i = file_offset h0 f in
+    	      	      	      let j = file_offset h0 f +^ len in
+			      modifies_1 s h0 h1 /\
+    	      	      	      file_state h1 f = FileOpen /\ 
+    	      	      	      file_offset h1 f = j /\
+			      file_content h0 f.stat = file_content h1 f.stat /\
+			      ((v i <= v f.stat.size /\ v j <= v f.stat.size) ==> s = file_sub h1 f i len) /\
+			      ((v i <= v f.stat.size /\ v j > v f.stat.size) ==>  sub s zero (f.stat.size -^ i) = file_sub h1 f i (f.stat.size -^ i))))
+			      
+
+val file_next_write_buffer: fb:buffer file_handle -> len:u64 -> Stack uint8_p
+    (requires (fun h0 -> v len <= v max_block_size /\
+    	      	         length fb = 1 /\ live h0 fb /\
+    	      	         (let f = get h0 fb 0 in
+			  file_state h0 f = FileOpen)))
+    (ensures  (fun h0 s h1 -> let f = get h1 fb 0 in
+    	      	              let i = file_offset h0 f in
+    	      	      	      let j = file_offset h0 f +^ len in
+			      modifies_1 s h0 h1 /\
+    	      	      	      file_state h1 f = FileOpen /\ 
+    	      	      	      file_offset h1 f = j /\
+			      file_content h0 f.stat = file_content h1 f.stat /\
+			      ((v i <= v f.stat.size /\ v j <= v f.stat.size) ==> s = file_sub h1 f i len) /\
+			      ((v i <= v f.stat.size /\ v j > v f.stat.size) ==>  sub s zero (f.stat.size -^ i) = file_sub h1 f i (f.stat.size -^ i))))
+			      
+
+val file_close: fb:buffer file_handle -> Stack bool
+    (requires (fun h0 -> length fb = 1 /\ live h0 fb /\
+                         (let f = get h0 fb 0 in
+			  file_state h0 f = FileOpen)))
+    (ensures  (fun h0 r h1 -> r ==> 
+                         (let f = get h1 fb 0 in
+       	      	      	  file_state h1 f = FileClosed /\
+    			  file_content h0 f.stat = file_content h1 f.stat)))
+
